finish uniformozation

coq/UntypedSemantics.v
@@ -1933,7 +1933,7 @@ Section Interp.
         end
       | URead prt idx =>
         if may_read sched_log prt idx then
-          Some (log_cons idx (LE Logs.LogRead prt (Bits 0 [])) action_log,
+          Some (log_cons idx (LE LogRead prt (Bits 0 [])) action_log,
             match prt with
             | P0 => REnv.(getenv) r idx
             | P1 =>
@@ -1951,7 +1951,7 @@ Section Interp.
           interp_action Gamma sched_log action_log v in
         if may_write sched_log action_log prt idx then
           Some (
-            log_cons idx (LE Logs.LogWrite prt val) action_log, Bits 0 [], Gamma
+            log_cons idx (LE LogWrite prt val) action_log, Bits 0 [], Gamma
           )
         else None
       | UUnop fn arg =>
@@ -2022,17 +2022,14 @@ Section Interp.
 
       Definition interp_cycle (s: scheduler pos_t rule_name_t) :=
         commit_update r (interp_scheduler s).
-
     End Scheduler.
-    End Action.
+  End Action.
 End Interp.
 
 Section Eq.
-
   Context {pos_t var_t fn_name_t reg_t ext_fn_t: Type}.
   Context {reg_t_eq_dec: EqDec reg_t}.
   Context {var_t_eq_dec: EqDec var_t}.
-
 
   Context {TR: reg_t -> type}.
   Context {Sigma: ext_fn_t -> ExternalSignature}.
@@ -2043,18 +2040,13 @@ Section Eq.
   Context (tsigma: forall f, Sig_denote (Sigma f)).
 
   Hypothesis tsigma_correct:
-    forall f v,
-      sigma f (val_of_value v) = val_of_value (tsigma f v).
+    forall f v, sigma f (val_of_value v) = val_of_value (tsigma f v).
 
   Definition env_t_R
-             {K: Type}
-             {V1 V2: K -> Type}
-             (R: forall k, V1 k -> V2 k -> Prop)
-             (e: Env K)
-             (e1: env_t e (fun x => V1 x))
-             (e2: env_t e (fun x => V2 x)) : Prop :=
-    forall k,
-      R k (getenv e e1 k) (getenv e e2 k).
+    {K: Type} {V1 V2: K -> Type} (R: forall k, V1 k -> V2 k -> Prop)
+    (e: Env K) (e1: env_t e (fun x => V1 x)) (e2: env_t e (fun x => V2 x))
+  : Prop :=
+    forall k, R k (getenv e e1 k) (getenv e e2 k).
 
   Definition logentry_eq
     {V:type} (ule: LogEntry val) (le: Logs.LogEntry V)
@@ -2478,6 +2470,116 @@ Section Eq.
     | USugar s => 0
     end.
 
+  Lemma interp_args_correct:
+    let PP := fun u : uaction =>
+      forall
+        (p : pos_t) (sig : tsig var_t) (tau : type)
+        (a : TypedSyntax.action pos_t var_t fn_name_t TR Sigma sig tau),
+      TypeInference.type_action TR Sigma p sig u =
+      Success
+        (existT (fun tau0 : type =>
+            TypedSyntax.action pos_t var_t fn_name_t TR Sigma sig tau0
+        ) tau a) ->
+      forall
+        (Gamma : TypedSemantics.tcontext sig) (UGamma : list (var_t * val)),
+      gamma_eq sig UGamma Gamma ->
+      forall
+        (sched_log action_log action_log' : Logs.Log TR REnv)
+        (usched_log uaction_log : env_t REnv (fun _ : reg_t => RLog val)),
+      log_eq REnv usched_log sched_log ->
+      log_eq REnv uaction_log action_log ->
+      forall (v : tau) (Gamma' : TypedSemantics.tcontext sig),
+      TypedSemantics.interp_action tr tsigma Gamma sched_log action_log a
+      = Some (action_log', v, Gamma') ->
+      exists (uaction_log' : Log) (UGamma' : list (var_t * val)),
+        interp_action r sigma UGamma usched_log uaction_log u
+        = Some (uaction_log', val_of_value v, UGamma')
+        /\ log_eq REnv uaction_log' action_log'
+        /\ gamma_eq sig UGamma' Gamma'
+    in
+    forall (l : list (var_t * type)) (args' : list uaction),
+    (forall arg : uaction, In arg args' -> PP arg) ->
+    forall
+      (p : pos_t) (sig : tsig var_t)
+      (s' : list {
+        tau : type & TypedSyntax.action pos_t var_t fn_name_t TR Sigma sig tau
+      }),
+    result_list_map (TypeInference.type_action TR Sigma p sig) args'
+    = Success s' ->
+    forall
+      (Gamma : TypedSemantics.tcontext sig) (UGamma : list (var_t * val)),
+    gamma_eq sig UGamma Gamma ->
+    forall
+      (sched_log action_log action_log' : Logs.Log TR REnv)
+      (usched_log uaction_log : env_t REnv (fun _ : reg_t => RLog val)),
+    log_eq REnv usched_log sched_log ->
+    log_eq REnv uaction_log action_log ->
+    forall
+      s0 : context (fun k_tau : var_t * type =>
+        TypedSyntax.action pos_t var_t fn_name_t TR Sigma sig (snd k_tau)
+      ) l,
+    assert_argtypes' l (combine (map (TypeInference.actpos p) args') s')
+    = Success s0 -> Datatypes.length args' = Datatypes.length s' ->
+    forall
+      (v : TypedSemantics.tcontext l)
+      (Gamma' : TypedSemantics.tcontext sig),
+    TypedSemantics.interp_args'
+      (@TypedSemantics.interp_action
+        pos_t var_t fn_name_t reg_t ext_fn_t TR Sigma REnv tr tsigma
+      ) Gamma sched_log action_log s0 = Some (action_log', v, Gamma')
+    -> exists
+      (uaction_log' : Log) (res : list val) (UGamma' : list (var_t * val)),
+    fold_right (
+      fun (a0 : uaction) (acc : option (Log * list val * list (var_t * val)))
+      =>
+        let/opt3 action_log0, l0, Gamma0 := acc in (
+          let/opt3 action_log1, v0, Gamma1 :=
+            interp_action r sigma Gamma0 usched_log action_log0 a0
+           in Some (action_log1, v0 :: l0, Gamma1)
+        )
+    ) (Some (uaction_log, [], UGamma)) args'
+    = Some (uaction_log', res, UGamma') /\
+    gamma_eq l (combine (map fst l) res) v /\
+    log_eq REnv uaction_log' action_log' /\ gamma_eq sig UGamma' Gamma'.
+  Proof.
+    induction l; simpl; intros.
+    - destr_in H4; [|now inv H4]. inv H4.
+      apply combine_nil_inv in Heql; eauto. destruct Heql. subst.
+      destruct args'; simpl in *; try congruence. inv H6.
+      eexists; eexists; eexists; repeat split; eauto.
+      constructor.
+      rewrite <- H5. rewrite map_length. auto.
+    - destr_in H4.
+      destr_in H4; [inv H4|].
+      destr_in H4.
+      destr_in H4; [|inv H4].
+      destr_in H4; [|inv H4]. inv H4.
+      destruct args'.
+      + simpl in Heql0. congruence.
+      + simpl in Heql0.
+        destr_in Heql0. congruence. inv Heql0. simpl in *.
+        unfold opt_bind in H6.
+        destr_in H6; [|inv H6]. destruct p0. destruct p0.
+        destr_in H6; [|inv H6]. destruct p0. destruct p0.
+        inv H6. simpl in *.
+        destr_in H0; [|inv H0].
+        destr_in H0; [|inv H0]. inv H0. simpl in *.
+        edestruct IHl as (ual' & res & ug' & EQ & Geq' & ALeq & Geq2').
+        intros; eapply H. right; apply H0.
+        apply Heqr3. 4: eauto.
+        5: apply Heqo. eauto. eauto. eauto. lia.
+        rewrite EQ. simpl.
+        destruct s; simpl in *.
+        apply cast_action_eq in Heqr0.
+        destruct Heqr0 as (pf & EQr0). subst.
+        simpl in Heqo0.
+        edestruct (H u) as (ual2' & ug2' & EQ2 & ALeq2 & Geq4'). auto. eauto.
+        4: eauto. eauto. eauto. eauto.
+        rewrite EQ2. simpl.
+        eexists; eexists; eexists; repeat split; eauto.
+        constructor. auto.
+  Qed.
+
   Lemma interp_action_correct:
     forall
       ua p sig tau a
@@ -2740,38 +2842,331 @@ Section Eq.
         rewrite rev_length; auto.
       }
       assert (
-          forall (p : pos_t) (sig : tsig var_t) s,
-            result_list_map (TypeInference.type_action TR Sigma p sig) args = Success s ->
-            forall (Gamma : TypedSemantics.tcontext sig) (UGamma : list (var_t * val)),
-              gamma_eq sig UGamma Gamma ->
-     forall (sched_log action_log action_log' : Logs.Log TR REnv)
-       (usched_log uaction_log : env_t REnv (fun _ : reg_t => RLog val)),
-     log_eq REnv usched_log sched_log ->
-     log_eq REnv uaction_log action_log ->
-     forall (s0 : context
-     (fun k_tau : var_t * type =>
-      TypedSyntax.action pos_t var_t fn_name_t TR Sigma sig (snd k_tau))
-     (rev (int_argspec ufn))),
-       assert_argtypes' (rev (int_argspec ufn))
-                        (rev (combine (map (TypeInference.actpos p) args) s)) = Success s0 ->
-       List.length args = List.length (rev s) ->
-     forall v (Gamma' : TypedSemantics.tcontext sig),
-       TypedSemantics.interp_args'
-         (@TypedSemantics.interp_action pos_t var_t fn_name_t reg_t ext_fn_t TR Sigma REnv tr tsigma)
-         Gamma sched_log action_log s0 =
-     Some (action_log', v, Gamma') ->
-     exists (uaction_log' : Log) res (UGamma' : list (var_t * val)),
-       fold_right
-      (fun a0 (acc : option (Log * list val * list (var_t * val))) =>
-       let/opt3 action_log0, l0, Gamma0 := acc
-       in (let/opt3 action_log1, v0, Gamma1
-           := interp_action r sigma Gamma0 usched_log action_log0 a0
-           in Some (action_log1, v0 :: l0, Gamma1))) (Some (uaction_log, [], UGamma)) (rev args) =
-       Some (uaction_log', res, UGamma') /\
-       gamma_eq _ (combine (map fst (rev (int_argspec ufn))) (res)) v /\
-       log_eq REnv uaction_log' action_log' /\ gamma_eq sig UGamma' Gamma').
+        forall (p : pos_t) (sig : tsig var_t) s,
+        result_list_map (TypeInference.type_action TR Sigma p sig) args
+        = Success s ->
+          forall
+            (Gamma : TypedSemantics.tcontext sig) (UGamma : list (var_t * val)),
+          gamma_eq sig UGamma Gamma ->
+          forall
+            (sched_log action_log action_log' : Logs.Log TR REnv)
+            (usched_log uaction_log : env_t REnv (fun _ : reg_t => RLog val)),
+          log_eq REnv usched_log sched_log ->
+          log_eq REnv uaction_log action_log ->
+          forall (s0 : context (fun k_tau : var_t * type =>
+            TypedSyntax.action pos_t var_t fn_name_t TR Sigma sig (snd k_tau)
+          ) (rev (int_argspec ufn))),
+          assert_argtypes'
+            (rev (int_argspec ufn))
+            (rev (combine (map (TypeInference.actpos p) args) s))
+          = Success s0 ->
+          List.length args = List.length (rev s) ->
+          forall v (Gamma' : TypedSemantics.tcontext sig),
+          TypedSemantics.interp_args' (
+            @TypedSemantics.interp_action
+              pos_t var_t fn_name_t reg_t ext_fn_t TR Sigma REnv tr tsigma
+          )
+          Gamma sched_log action_log s0
+          = Some (action_log', v, Gamma') ->
+          exists (uaction_log' : Log) res (UGamma' : list (var_t * val)),
+          fold_right (
+            fun a0
+              (acc : option (Log * list val * list (var_t * val))) =>
+                let/opt3 action_log0, l0, Gamma0 := acc in (
+                  let/opt3 action_log1, v0, Gamma1 :=
+                    interp_action r sigma Gamma0 usched_log action_log0 a0
+                  in
+                  Some (action_log1, v0 :: l0, Gamma1)
+                )
+          ) (Some (uaction_log, [], UGamma)) (rev args)
+          = Some (uaction_log', res, UGamma')
+          /\ gamma_eq _ (combine (map fst (rev (int_argspec ufn))) (res)) v
+          /\ log_eq REnv uaction_log' action_log'
+          /\ gamma_eq sig UGamma' Gamma'
+      ).
       {
         clear - IHua.
+        rewrite <- (rev_involutive args).
+        assert (IHua': forall arg, In arg (rev args) -> PP arg).
+        {
+          intros.
+          eapply IHua.
+          apply In_rev in H.
+          revert arg H.
+          induction args; simpl; intros; eauto. easy.
+          destruct H. subst. lia.
+          eapply IHargs in H. lia. intros. eapply IHua. simpl. lia.
+        }
+        clear IHua. revert IHua'.
+        generalize (rev args) as args'.
+        intros args' IHua' p sig s RLM.
+        apply result_list_map_rev in RLM.
+        rewrite combine_rev.
+        rewrite map_rev. rewrite rev_involutive.
+        revert RLM. rewrite rev_involutive.
+        generalize (rev s) as s'. clear s.
+        rewrite rev_length.
+        revert args' IHua' p sig.
+        generalize (rev (int_argspec ufn)). clear args.
+        apply interp_args_correct.
+        - rewrite map_length.
+          apply result_list_map_length in RLM.
+          rewrite ! rev_length in *. auto.
+      }
+      edestruct H0 as (uaction_log' & res & UGamma' & FR & Geq1 & ALeq & Geq2).
+      eauto. 4: eauto. 5: eauto. eauto. eauto. eauto. auto.
+      rewrite fold_left_rev_right in FR.
+      setoid_rewrite FR. simpl.
+      clear H0 FR.
+      edestruct (IHua (int_body ufn)) as (ual' & g' & IA' & ALeq2 & Geq). lia. eauto.
+      eauto. 3: eauto. eauto. eauto.
+      erewrite combine_map.
+      rewrite IA'. simpl.
+      eexists; eexists; repeat split; eauto.
+      simpl; reflexivity.
+    - destr_in TA; [|inv TA].
+      inv TA.
+      apply Eqdep_dec.inj_pair2_eq_dec in H2. 2: apply eq_dec. subst. simpl in H.
+      destruct s. simpl in *.
+      edestruct (IHua ua) as (ual' & g' & IA' & ALeq & Geq). lia. eauto.
+      4: apply H. eauto. eauto. eauto.
+      rewrite IA'.
+      eexists; eexists; repeat split; eauto.
+    - inv TA.
+  Qed.
+
+  Lemma interp_action_none:
+    forall
+      ua p sig tau a (TA:
+        TypeInference.type_action TR Sigma p sig ua = Success (existT _ tau a)
+      ) (Gamma: TypedSemantics.tcontext sig) (UGamma: list (var_t * val))
+      (GammaEq: gamma_eq sig UGamma Gamma) sched_log action_log usched_log
+      uaction_log (SL: log_eq REnv usched_log sched_log)
+      (AL: log_eq REnv uaction_log action_log)
+    ,
+    TypedSemantics.interp_action tr tsigma Gamma sched_log action_log a = None
+    ->
+    interp_action
+      (pos_t:=pos_t) (fn_name_t := fn_name_t) r sigma UGamma usched_log
+      uaction_log ua = None.
+  Proof.
+    intros ua. pattern ua.
+    match goal with
+    | |- ?P ua => set (PP:=P)
+    end.
+    remember (size_uaction ua).
+    revert ua Heqn.
+    pattern n.
+    eapply Nat.strong_right_induction with (z:=0).
+    { red. red. intros. subst. tauto. } 2: lia.
+    intros n0 _ Plt ua Heqn. subst.
+    assert (Plt': forall a, size_uaction a < size_uaction ua -> PP a).
+    { intros. eapply Plt. 3: reflexivity. lia. auto. }
+    clear Plt. rename Plt' into IHua. clear n. unfold PP.
+    destruct ua; simpl; intros; auto.
+    - destr_in TA; inv TA.
+      apply Eqdep_dec.inj_pair2_eq_dec in H2. 2: apply eq_dec. subst.
+      simpl in H. inv H.
+    - inv TA.
+      apply Eqdep_dec.inj_pair2_eq_dec in H2. 2: apply eq_dec. subst.
+      simpl in H. inv H.
+    - destr_in TA; [|inv TA].
+      destr_in TA; [|inv TA].
+      destr_in TA; [|inv TA]. inv TA.
+      apply Eqdep_dec.inj_pair2_eq_dec in H2. 2: apply eq_dec.
+      subst. simpl in H.
+      unfold opt_bind in H.
+      repeat destr_in H; [inv H|].
+      unfold opt_result in Heqr0; destr_in Heqr0; inv Heqr0.
+      destruct s. simpl in *.
+      destruct s0. simpl in *.
+      apply cast_action_eq in Heqr2.
+      destruct Heqr2 as (pf & EQ). subst.
+      simpl in Heqo.
+      erewrite IHua; eauto.
+    - destr_in TA; [|inv TA].
+      destr_in TA; [|inv TA].
+      destr_in TA; [|inv TA]. inv TA.
+      apply Eqdep_dec.inj_pair2_eq_dec in H2. 2: apply eq_dec.
+      subst. simpl in H.
+      destruct s; simpl in *.
+      apply cast_action_eq in Heqr1.
+      destruct Heqr1 as (pf & EQ). subst.
+      simpl in H.
+      unfold opt_bind in H.
+      repeat destr_in H.
+      edestruct interp_action_correct as (ual' & g' & IA' & ALeq & Geq). eauto.
+      4: eauto. eauto. eauto. eauto. rewrite IA'. simpl.
+      destruct s1. simpl in *.
+      erewrite IHua; eauto. lia.
+      erewrite IHua; eauto. simpl; lia.
+    - destr_in TA; [|inv TA].
+      destr_in TA; [|inv TA].
+      inv TA.
+      apply Eqdep_dec.inj_pair2_eq_dec in H2. 2: apply eq_dec.
+      subst. simpl in H.
+      destruct s, s0. simpl in *.
+      unfold opt_bind in H.
+      repeat destr_in H; try (now inv H).
+      edestruct (interp_action_correct ua1) as (ual' & g' & IA' & ALeq & Geq).
+      eauto.
+      4: apply Heqo. eauto. eauto. eauto.
+      rewrite IA'. simpl.
+      erewrite IHua; eauto. lia.
+      constructor; eauto.
+      erewrite IHua; eauto. lia.
+    - destr_in TA; [|inv TA].
+      destr_in TA; [|inv TA].
+      destr_in TA; [|inv TA].
+      destr_in TA; [|inv TA].
+      destr_in TA; [|inv TA].
+      inv TA.
+      apply Eqdep_dec.inj_pair2_eq_dec in H2. 2: apply eq_dec.
+      subst. simpl in H.
+      destruct s. simpl in *.
+      apply cast_action_eq in Heqr1.
+      destruct Heqr1 as (pf & EQ). subst.
+      simpl in H.
+      destruct s1, s2. simpl in *.
+      apply cast_action_eq in Heqr4.
+      destruct Heqr4 as (pf & EQ). subst.
+      simpl in H.
+      unfold opt_bind in H.
+      destr_in H. destruct p0. destruct p0.
+      edestruct (interp_action_correct ua1) as (ual' & g' & IA' & ALeq & Geq).
+      eauto.
+      4: apply Heqo. eauto. eauto. eauto.
+      rewrite IA'. simpl.
+      destr_in H.
+      erewrite IHua; eauto. lia.
+      erewrite IHua; eauto. lia.
+      erewrite IHua; eauto. lia.
+    - inv TA.
+      apply Eqdep_dec.inj_pair2_eq_dec in H2. 2: apply eq_dec.
+      subst. simpl in H.
+      erewrite may_read_eq in H; eauto.
+      destr_in H; [inv H|]. auto.
+    - destr_in TA; [|inv TA].
+      destr_in TA; [|inv TA].
+      inv TA.
+      apply Eqdep_dec.inj_pair2_eq_dec in H2. 2: apply eq_dec.
+      subst. simpl in H.
+      destruct s. simpl in *.
+      apply cast_action_eq in Heqr1.
+      destruct Heqr1 as (pf & EQ). subst.
+      simpl in H.
+      unfold opt_bind in H.
+      destr_in H.
+      + destruct p0. destruct p0.
+        edestruct (interp_action_correct ua) as (ual' & g' & IA' & ALeq & Geq).
+        eauto.
+        4: apply Heqo. eauto. eauto. eauto.
+        rewrite IA'. simpl.
+        erewrite may_write_eq in H; eauto.
+        destr_in H; inv H. auto.
+      + erewrite IHua; eauto.
+    - destr_in TA; [|inv TA].
+      destr_in TA; [|inv TA].
+      destr_in TA; [|inv TA].
+      inv TA.
+      apply Eqdep_dec.inj_pair2_eq_dec in H2. 2: apply eq_dec.
+      subst. simpl in H.
+      destruct s. simpl in *.
+      apply cast_action_eq in Heqr2.
+      destruct Heqr2 as (pf & EQ). subst.
+      simpl in H.
+      unfold opt_bind in H.
+      repeat destr_in H; inv H.
+      erewrite IHua; eauto.
+    - destr_in TA; [|inv TA].
+      destr_in TA; [|inv TA].
+      destr_in TA; [|inv TA].
+      destr_in TA; [|inv TA].
+      destr_in TA; [|inv TA].
+      inv TA.
+      apply Eqdep_dec.inj_pair2_eq_dec in H2. 2: apply eq_dec.
+      subst. simpl in H.
+      destruct s, s0. simpl in *.
+      apply cast_action_eq in Heqr3.
+      destruct Heqr3 as (pf & EQ). subst.
+      apply cast_action_eq in Heqr4.
+      destruct Heqr4 as (pf & EQ). subst.
+      simpl in H.
+      unfold opt_bind in H.
+      repeat destr_in H; inv H.
+      edestruct (interp_action_correct ua1) as (ual' & g' & IA' & ALeq & Geq).
+      eauto.
+      4: apply Heqo. eauto. eauto. eauto.
+      rewrite IA'. simpl.
+      erewrite IHua; eauto. lia.
+      erewrite IHua; eauto. lia.
+    - destr_in TA; [|inv TA].
+      destr_in TA; [|inv TA].
+      inv TA.
+      apply Eqdep_dec.inj_pair2_eq_dec in H2. 2: apply eq_dec.
+      subst. simpl in H.
+      destruct s. simpl in *.
+      apply cast_action_eq in Heqr1.
+      destruct Heqr1 as (pf & EQ). subst.
+      simpl in H.
+      unfold opt_bind in H.
+      repeat destr_in H; [inv H|].
+      erewrite IHua; eauto.
+    - destr_in TA; [|inv TA].
+      destr_in TA; [|inv TA].
+      destr_in TA; [|inv TA].
+      destr_in TA; [|inv TA].
+      inv TA.
+      apply Eqdep_dec.inj_pair2_eq_dec in H2. 2: apply eq_dec.
+      subst. simpl in H.
+      destruct s1. simpl in *.
+      apply cast_action_eq in Heqr3.
+      destruct Heqr3 as (pf & EQ). subst.
+      simpl in H.
+      unfold TypeInference.assert_argtypes in Heqr1.
+      rewrite assert_argtypes'_eq in Heqr1.
+      assert (List.length args = List.length (rev s)).
+      {
+        apply result_list_map_length in Heqr0. rewrite <- Heqr0.
+        rewrite rev_length; auto.
+      }
+      assert (
+        forall (p : pos_t) (sig : tsig var_t) s,
+        result_list_map (TypeInference.type_action TR Sigma p sig) args
+        = Success s ->
+        forall
+          (Gamma : TypedSemantics.tcontext sig) (UGamma : list (var_t * val)),
+        gamma_eq sig UGamma Gamma ->
+        forall (sched_log action_log action_log' : Logs.Log TR REnv)
+        (usched_log uaction_log : env_t REnv (fun _ : reg_t => RLog val)),
+        log_eq REnv usched_log sched_log ->
+        log_eq REnv uaction_log action_log ->
+        forall (
+          s0 : context
+          (fun k_tau : var_t * type =>
+            TypedSyntax.action pos_t var_t fn_name_t TR Sigma sig (snd k_tau)
+          ) (rev (int_argspec ufn))
+        ),
+        assert_argtypes'
+          (rev (int_argspec ufn))
+          (rev (combine (map (TypeInference.actpos p) args) s))
+        = Success s0 ->
+        List.length args = List.length (rev s) ->
+        TypedSemantics.interp_args' (@TypedSemantics.interp_action
+          pos_t var_t fn_name_t reg_t ext_fn_t TR Sigma REnv tr tsigma
+        ) Gamma sched_log action_log s0 = None ->
+        fold_right (
+          fun a0 (acc : option (Log * list val * list (var_t * val))) =>
+            let/opt3 action_log0, l0, Gamma0 := acc in (
+              let/opt3 action_log1, v0, Gamma1 :=
+                interp_action r sigma Gamma0 usched_log action_log0 a0 in
+              Some (action_log1, v0 :: l0, Gamma1)
+            )
+        ) (Some (uaction_log, [], UGamma)) (rev args) = None
+      ).
+      {
+        generalize interp_action_correct as IAC. intro IAC.
+        clear - IHua IAC.
         rewrite <- (rev_involutive args).
         assert (IHua': forall arg, In arg (rev args) -> PP arg).
         {
@@ -2793,556 +3188,170 @@ Section Eq.
         rewrite rev_length.
         revert args' IHua' p sig.
         generalize (rev (int_argspec ufn)). clear args.
+        induction l; simpl; intros.
+        - destr_in H2; [|now inv H2]. inv H2.
+          apply combine_nil_inv in Heql; eauto. destruct Heql. subst.
+          destruct args'; simpl in *; try congruence. inv H4.
+        - destr_in H2.
+          destr_in H2; [inv H2|].
+          destr_in H2.
+          destr_in H2; [|inv H2].
+          destr_in H2; [|inv H2]. inv H2.
+          destruct args'.
+          + simpl in Heql0. congruence.
+          + simpl in Heql0.
+            destr_in Heql0. congruence. inv Heql0. simpl in *.
+            unfold opt_bind in H4.
+            destr_in RLM; [|inv RLM].
+            destr_in RLM; [|inv RLM]. inv RLM. simpl in *.
+            destr_in H4. destruct p0. destruct p0.
+            * edestruct interp_args_correct as (
+                ual' & res & ug' & FR & Geq & Leq & Geq2
+              ).
+              intros arg IN. intros; eapply IAC.  12: eauto. all:eauto.
+              rewrite FR. simpl.
+              repeat destr_in H4. inv H4.
+              destruct s. simpl in *. erewrite IHua'; simpl; eauto.
+              apply cast_action_eq in Heqr0. destruct Heqr0 as (pf & EQ).
+              subst. simpl in *. eauto.
+            * erewrite IHl; simpl; eauto.
+        - rewrite map_length.
+          apply result_list_map_length in RLM.
+          rewrite ! rev_length in *. auto.
+      }
+      move H at bottom.
+      unfold opt_bind in H.
+      repeat destr_in H; try inv H.
+      * rewrite combine_rev in Heqr1.
+        rewrite <- map_rev in Heqr1.
+        edestruct interp_args_correct as (
+          ual' & res & ug' & FR & Geq & Leq & Geq2
+        ).
+        intros arg IN. intros; eapply interp_action_correct. 10:eauto.
+        6: apply result_list_map_rev; eauto. 5: eauto. 9: eauto. all: eauto.
+        rewrite rev_length; auto.
+        rewrite <- fold_left_rev_right. setoid_rewrite FR. simpl.
+        erewrite IHua; simpl; eauto. lia.
+        erewrite combine_map. eauto. reflexivity.
+        rewrite map_length. rewrite H0.
+        rewrite rev_length; auto.
+      * rewrite <- fold_left_rev_right.
+        erewrite H1. reflexivity. 6: eauto. eauto. eauto. all: eauto.
+    - destr_in TA; [|inv TA].
+      inv TA.
+      apply Eqdep_dec.inj_pair2_eq_dec in H2. 2: apply eq_dec.
+      subst. simpl in H.
+      destruct s. simpl in *.
+      eapply IHua; eauto.
+  Qed.
 
-            Lemma interp_args_correct:
-              let PP := fun u : uaction =>
-                                forall (p : pos_t) (sig : tsig var_t) (tau : type)
-                                       (a : TypedSyntax.action pos_t var_t fn_name_t TR Sigma sig tau),
-                                  TypeInference.type_action TR Sigma p sig u =
-                                  Success
-                                    (existT (fun tau0 : type => TypedSyntax.action pos_t var_t fn_name_t TR Sigma sig tau0) tau
-                                            a) ->
-                                  forall (Gamma : TypedSemantics.tcontext sig) (UGamma : list (var_t * val)),
-                                    gamma_eq sig UGamma Gamma ->
-                                    forall (sched_log action_log action_log' : Logs.Log TR REnv)
-                                           (usched_log uaction_log : env_t REnv (fun _ : reg_t => RLog val)),
-                                      log_eq REnv usched_log sched_log ->
-                                      log_eq REnv uaction_log action_log ->
-                                      forall (v : tau) (Gamma' : TypedSemantics.tcontext sig),
-                                        TypedSemantics.interp_action tr tsigma Gamma sched_log action_log a =
-                                        Some (action_log', v, Gamma') ->
-                                        exists (uaction_log' : Log) (UGamma' : list (var_t * val)),
-                                          interp_action r sigma UGamma usched_log uaction_log u =
-                                          Some (uaction_log', val_of_value v, UGamma') /\
-                                          log_eq REnv uaction_log' action_log' /\ gamma_eq sig UGamma' Gamma'  in
-              forall (l : list (var_t * type)) (args' : list uaction),
-                (forall arg : uaction, In arg args' -> PP arg) ->
-                forall (p : pos_t) (sig : tsig var_t)
-                       (s' : list {tau : type & TypedSyntax.action pos_t var_t fn_name_t TR Sigma sig tau}),
-                  result_list_map (TypeInference.type_action TR Sigma p sig) args' = Success s' ->
-                  forall (Gamma : TypedSemantics.tcontext sig) (UGamma : list (var_t * val)),
-                    gamma_eq sig UGamma Gamma ->
-                    forall (sched_log action_log action_log' : Logs.Log TR REnv)
-                           (usched_log uaction_log : env_t REnv (fun _ : reg_t => RLog val)),
-                      log_eq REnv usched_log sched_log ->
-                      log_eq REnv uaction_log action_log ->
-                      forall
-                        s0 : context
-                               (fun k_tau : var_t * type =>
-                                  TypedSyntax.action pos_t var_t fn_name_t TR Sigma sig (snd k_tau)) l,
-                        assert_argtypes' l (combine (map (TypeInference.actpos p) args') s') = Success s0 ->
-                        Datatypes.length args' = Datatypes.length s' ->
-                        forall (v : TypedSemantics.tcontext l) (Gamma' : TypedSemantics.tcontext sig),
-                          TypedSemantics.interp_args'
-                            (@TypedSemantics.interp_action pos_t var_t fn_name_t reg_t ext_fn_t TR Sigma REnv tr tsigma) Gamma
-                            sched_log action_log s0 = Some (action_log', v, Gamma') ->
-                          exists (uaction_log' : Log) (res : list val) (UGamma' : list (var_t * val)),
-                            fold_right
-                              (fun (a0 : uaction) (acc : option (Log * list val * list (var_t * val))) =>
-                                 let/opt3 action_log0, l0, Gamma0 := acc
-                                 in (let/opt3 action_log1, v0, Gamma1 := interp_action r sigma Gamma0 usched_log action_log0 a0
-                                     in Some (action_log1, v0 :: l0, Gamma1))) (Some (uaction_log, [], UGamma)) args' =
-                            Some (uaction_log', res, UGamma') /\
-                            gamma_eq l (combine (map fst l) res) v /\
-                            log_eq REnv uaction_log' action_log' /\ gamma_eq sig UGamma' Gamma'.
-            Proof.
-              induction l; simpl; intros.
-              - destr_in H4; [|now inv H4]. inv H4.
-                apply combine_nil_inv in Heql; eauto. destruct Heql. subst.
-                destruct args'; simpl in *; try congruence. inv H6.
-                eexists; eexists; eexists; repeat split; eauto.
-                constructor.
-                rewrite <- H5. rewrite map_length. auto.
-              - destr_in H4.
-                destr_in H4; [inv H4|].
-                destr_in H4.
-                destr_in H4; [|inv H4].
-                destr_in H4; [|inv H4]. inv H4.
-                destruct args'.
-                + simpl in Heql0. congruence.
-                + simpl in Heql0.
-                  destr_in Heql0. congruence. inv Heql0. simpl in *.
-                  unfold opt_bind in H6.
-                  destr_in H6; [|inv H6]. destruct p0. destruct p0.
-                  destr_in H6; [|inv H6]. destruct p0. destruct p0.
-                  inv H6. simpl in *.
-                  destr_in H0; [|inv H0].
-                  destr_in H0; [|inv H0]. inv H0. simpl in *.
-                  edestruct IHl as (ual' & res & ug' & EQ & Geq' & ALeq & Geq2').
-                  intros; eapply H. right; apply H0.
-                  apply Heqr3. 4: eauto.
-                  5: apply Heqo. eauto. eauto. eauto. lia.
+  Lemma log_eq_empty: log_eq REnv log_empty Logs.log_empty.
+  Proof.
+    repeat red.
+    unfold log_empty, Logs.log_empty.
+    intros; repeat rewrite getenv_create. constructor.
+  Qed.
 
-                  rewrite EQ. simpl.
+  Lemma interp_rule_correct:
+    forall
+      ua p rl (TA: TypeInference.tc_rule TR Sigma p ua = Success rl)
+      sched_log usched_log (SL: log_eq REnv usched_log sched_log) action_log,
+    TypedSemantics.interp_rule tr tsigma sched_log rl = Some (action_log) ->
+    exists uaction_log,
+    interp_rule (pos_t:=pos_t) (fn_name_t := fn_name_t) r sigma usched_log ua
+    = Some (uaction_log) /\ log_eq REnv uaction_log action_log.
+  Proof.
+    intros.
+    unfold TypeInference.tc_rule in TA.
+    unfold TypeInference.tc_action in TA.
+    destr_in TA; [|inv TA].
+    destruct s; simpl in *.
+    apply cast_action_eq in TA. destruct TA as (pp & EQ).
+    subst. simpl in *.
+    unfold TypedSemantics.interp_rule in H.
+    destr_in H; [|inv H].
+    destruct p0. destruct p0. inv H.
+    unfold interp_rule.
+    edestruct interp_action_correct as (ual' & ug' & IA & LE & GE).
+    eauto. constructor. 3: eauto. apply SL.
+    apply log_eq_empty.
+    rewrite IA.
+    eexists; split; eauto.
+  Qed.
 
-                  destruct s; simpl in *.
-                  apply cast_action_eq in Heqr0.
-                  destruct Heqr0 as (pf & EQr0). subst.
-                  simpl in Heqo0.
+  Lemma interp_rule_none:
+    forall
+      ua p rl (TA: TypeInference.tc_rule TR Sigma p ua = Success rl)
+      sched_log usched_log (SL: log_eq REnv usched_log sched_log),
+    TypedSemantics.interp_rule tr tsigma sched_log rl = None ->
+    interp_rule (pos_t:=pos_t) (fn_name_t := fn_name_t) r sigma usched_log ua
+    = None.
+  Proof.
+    intros.
+    unfold TypeInference.tc_rule in TA.
+    unfold TypeInference.tc_action in TA.
+    destr_in TA; [|inv TA].
+    destruct s; simpl in *.
+    apply cast_action_eq in TA. destruct TA as (pp & EQ).
+    subst. simpl in *.
+    unfold TypedSemantics.interp_rule in H.
+    repeat destr_in H; [inv H|].
+    unfold interp_rule.
+    erewrite interp_action_none; eauto. constructor.
+    apply log_eq_empty.
+  Qed.
 
-                  edestruct (H u) as (ual2' & ug2' & EQ2 & ALeq2 & Geq4'). auto. eauto.
-                  4: eauto. eauto. eauto. eauto.
-                  rewrite EQ2. simpl.
-                  eexists; eexists; eexists; repeat split; eauto.
-                  constructor. auto.
-            Qed.
-            apply interp_args_correct.
-            - rewrite map_length.
-              apply result_list_map_length in RLM.
-              rewrite ! rev_length in *. auto.
-          }
-          edestruct H0 as (uaction_log' & res & UGamma' & FR & Geq1 & ALeq & Geq2).
-          eauto. 4: eauto. 5: eauto. eauto. eauto. eauto. auto.
-          rewrite fold_left_rev_right in FR.
-          setoid_rewrite FR. simpl.
-          clear H0 FR.
-          edestruct (IHua (int_body ufn)) as (ual' & g' & IA' & ALeq2 & Geq). lia. eauto.
-          eauto. 3: eauto. eauto. eauto.
+  Context {rule_name_t: Type}.
 
-          erewrite combine_map.
-          rewrite IA'. simpl.
-          eexists; eexists; repeat split; eauto.
-          simpl; reflexivity.
+  Lemma interp_scheduler'_correct:
+    forall
+      (urules: rule_name_t -> uaction)
+      (rules: rule_name_t -> TypedSyntax.rule pos_t var_t fn_name_t TR Sigma)
+      (TC: forall rnt, exists p,
+        TypeInference.tc_rule TR Sigma p (urules rnt) = Success (rules rnt)
+      ),
+    forall s l1 ul1 l2, log_eq REnv ul1 l1 ->
+      TypedSemantics.interp_scheduler' tr tsigma rules l1 s = l2 ->
+    exists ul2,
+      interp_scheduler' r sigma urules ul1 s = ul2 /\ log_eq REnv ul2 l2.
+  Proof.
+    induction s; simpl; intros; eauto.
+    - subst. eexists; split; eauto.
+    - destr_in H0.
+      + destruct (TC r0) as (p & TCR).
+        edestruct interp_rule_correct as (l' & EQ1 & EQ2). eauto. 2: eauto.
+        eauto.
+        rewrite EQ1.
+        eapply IHs; eauto.
+        apply log_eq_app; auto.
+      + destruct (TC r0) as (p & TCR).
+        erewrite interp_rule_none; eauto.
+    - destr_in H0.
+      + destruct (TC r0) as (p & TCR).
+        edestruct interp_rule_correct as (l' & EQ1 & EQ2). eauto. 2: eauto.
+        eauto.
+        rewrite EQ1.
+        eapply IHs1; eauto.
+        apply log_eq_app; auto.
+      + destruct (TC r0) as (p & TCR).
+        erewrite interp_rule_none; eauto.
+  Qed.
 
-        - destr_in TA; [|inv TA].
-          inv TA.
-          apply Eqdep_dec.inj_pair2_eq_dec in H2. 2: apply eq_dec. subst. simpl in H.
-          destruct s. simpl in *.
-          edestruct (IHua ua) as (ual' & g' & IA' & ALeq & Geq). lia. eauto.
-          4: apply H. eauto. eauto. eauto.
-          rewrite IA'.
-          eexists; eexists; repeat split; eauto.
-        - inv TA.
-      Qed.
-
-
-      Lemma interp_action_none:
-        forall ua p sig tau a
-               (TA: TypeInference.type_action TR Sigma p sig ua = Success (existT _ tau a))
-               (Gamma: TypedSemantics.tcontext sig)
-               (UGamma: list (var_t * val))
-               (GammaEq: gamma_eq sig UGamma Gamma)
-               sched_log action_log
-               usched_log uaction_log
-               (SL: log_eq REnv usched_log sched_log)
-               (AL: log_eq REnv uaction_log action_log)
-        ,
-          TypedSemantics.interp_action
-            tr tsigma
-            Gamma sched_log action_log a = None ->
-            interp_action
-              (pos_t:=pos_t)
-              (fn_name_t := fn_name_t)
-              r sigma UGamma usched_log uaction_log ua = None
-      .
-      Proof.
-        intros ua. pattern ua.
-        match goal with
-        | |- ?P ua => set (PP:=P)
-        end.
-        remember (size_uaction ua).
-        revert ua Heqn.
-        pattern n.
-        eapply Nat.strong_right_induction with (z:=0).
-        {
-          red. red. intros. subst. tauto.
-        } 2: lia.
-        intros n0 _ Plt ua Heqn. subst.
-        assert (Plt':
-                  forall a,
-                    size_uaction a < size_uaction ua -> PP a
-               ).
-        {
-          intros. eapply Plt. 3: reflexivity. lia. auto.
-        } clear Plt.
-        rename Plt' into IHua. clear n. unfold PP.
-        destruct ua; simpl; intros; auto.
-        - destr_in TA; inv TA.
-          apply Eqdep_dec.inj_pair2_eq_dec in H2. 2: apply eq_dec. subst.
-          simpl in H. inv H.
-        - inv TA.
-          apply Eqdep_dec.inj_pair2_eq_dec in H2. 2: apply eq_dec. subst.
-          simpl in H. inv H.
-        - destr_in TA; [|inv TA].
-          destr_in TA; [|inv TA].
-          destr_in TA; [|inv TA]. inv TA.
-          apply Eqdep_dec.inj_pair2_eq_dec in H2. 2: apply eq_dec. subst. simpl in H.
-          unfold opt_bind in H.
-          repeat destr_in H; [inv H|].
-          unfold opt_result in Heqr0; destr_in Heqr0; inv Heqr0. destruct s. simpl in *.
-          destruct s0. simpl in *.
-          apply cast_action_eq in Heqr2.
-          destruct Heqr2 as (pf & EQ). subst.
-          simpl in Heqo.
-          erewrite IHua; eauto.
-        - destr_in TA; [|inv TA].
-          destr_in TA; [|inv TA].
-          destr_in TA; [|inv TA]. inv TA.
-          apply Eqdep_dec.inj_pair2_eq_dec in H2. 2: apply eq_dec. subst. simpl in H.
-          destruct s; simpl in *.
-          apply cast_action_eq in Heqr1.
-          destruct Heqr1 as (pf & EQ). subst.
-          simpl in H.
-          unfold opt_bind in H.
-          repeat destr_in H.
-          edestruct interp_action_correct as (ual' & g' & IA' & ALeq & Geq). eauto.
-          4: eauto. eauto. eauto. eauto. rewrite IA'. simpl.
-          destruct s1. simpl in *.
-          erewrite IHua; eauto. lia.
-          erewrite IHua; eauto. simpl; lia.
-        - destr_in TA; [|inv TA].
-          destr_in TA; [|inv TA].
-          inv TA.
-          apply Eqdep_dec.inj_pair2_eq_dec in H2. 2: apply eq_dec. subst. simpl in H.
-          destruct s, s0. simpl in *.
-          unfold opt_bind in H.
-          repeat destr_in H; try (now inv H).
-          edestruct (interp_action_correct ua1) as (ual' & g' & IA' & ALeq & Geq). eauto.
-          4: apply Heqo. eauto. eauto. eauto.
-          rewrite IA'. simpl.
-          erewrite IHua; eauto. lia.
-          constructor; eauto.
-          erewrite IHua; eauto. lia.
-        - destr_in TA; [|inv TA].
-          destr_in TA; [|inv TA].
-          destr_in TA; [|inv TA].
-          destr_in TA; [|inv TA].
-          destr_in TA; [|inv TA].
-          inv TA.
-          apply Eqdep_dec.inj_pair2_eq_dec in H2. 2: apply eq_dec. subst. simpl in H.
-          destruct s. simpl in *.
-          apply cast_action_eq in Heqr1.
-          destruct Heqr1 as (pf & EQ). subst.
-          simpl in H.
-          destruct s1, s2. simpl in *.
-          apply cast_action_eq in Heqr4.
-          destruct Heqr4 as (pf & EQ). subst.
-          simpl in H.
-          unfold opt_bind in H.
-          destr_in H. destruct p0. destruct p0.
-          edestruct (interp_action_correct ua1) as (ual' & g' & IA' & ALeq & Geq). eauto.
-          4: apply Heqo. eauto. eauto. eauto.
-          rewrite IA'. simpl.
-          destr_in H.
-          erewrite IHua; eauto. lia.
-          erewrite IHua; eauto. lia.
-          erewrite IHua; eauto. lia.
-        - inv TA.
-          apply Eqdep_dec.inj_pair2_eq_dec in H2. 2: apply eq_dec. subst. simpl in H.
-          erewrite may_read_eq in H; eauto.
-          destr_in H; [inv H|]. auto.
-        - destr_in TA; [|inv TA].
-          destr_in TA; [|inv TA].
-          inv TA.
-          apply Eqdep_dec.inj_pair2_eq_dec in H2. 2: apply eq_dec. subst. simpl in H.
-          destruct s. simpl in *.
-          apply cast_action_eq in Heqr1.
-          destruct Heqr1 as (pf & EQ). subst.
-          simpl in H.
-          unfold opt_bind in H.
-          destr_in H.
-          + destruct p0. destruct p0.
-            edestruct (interp_action_correct ua) as (ual' & g' & IA' & ALeq & Geq). eauto.
-            4: apply Heqo. eauto. eauto. eauto.
-            rewrite IA'. simpl.
-            erewrite may_write_eq in H; eauto.
-            destr_in H; inv H. auto.
-          + erewrite IHua; eauto.
-        - destr_in TA; [|inv TA].
-          destr_in TA; [|inv TA].
-          destr_in TA; [|inv TA].
-          inv TA.
-          apply Eqdep_dec.inj_pair2_eq_dec in H2. 2: apply eq_dec. subst. simpl in H.
-          destruct s. simpl in *.
-          apply cast_action_eq in Heqr2.
-          destruct Heqr2 as (pf & EQ). subst.
-          simpl in H.
-          unfold opt_bind in H.
-          repeat destr_in H; inv H.
-          erewrite IHua; eauto.
-        - destr_in TA; [|inv TA].
-          destr_in TA; [|inv TA].
-          destr_in TA; [|inv TA].
-          destr_in TA; [|inv TA].
-          destr_in TA; [|inv TA].
-          inv TA.
-          apply Eqdep_dec.inj_pair2_eq_dec in H2. 2: apply eq_dec. subst. simpl in H.
-          destruct s, s0. simpl in *.
-          apply cast_action_eq in Heqr3.
-          destruct Heqr3 as (pf & EQ). subst.
-          apply cast_action_eq in Heqr4.
-          destruct Heqr4 as (pf & EQ). subst.
-          simpl in H.
-          unfold opt_bind in H.
-          repeat destr_in H; inv H.
-          edestruct (interp_action_correct ua1) as (ual' & g' & IA' & ALeq & Geq). eauto.
-          4: apply Heqo. eauto. eauto. eauto.
-          rewrite IA'. simpl.
-          erewrite IHua; eauto. lia.
-          erewrite IHua; eauto. lia.
-        - destr_in TA; [|inv TA].
-          destr_in TA; [|inv TA].
-          inv TA.
-          apply Eqdep_dec.inj_pair2_eq_dec in H2. 2: apply eq_dec. subst. simpl in H.
-          destruct s. simpl in *.
-          apply cast_action_eq in Heqr1.
-          destruct Heqr1 as (pf & EQ). subst.
-          simpl in H.
-          unfold opt_bind in H.
-          repeat destr_in H; [inv H|].
-          erewrite IHua; eauto.
-        - destr_in TA; [|inv TA].
-          destr_in TA; [|inv TA].
-          destr_in TA; [|inv TA].
-          destr_in TA; [|inv TA].
-          inv TA.
-          apply Eqdep_dec.inj_pair2_eq_dec in H2. 2: apply eq_dec. subst. simpl in H.
-          destruct s1. simpl in *.
-          apply cast_action_eq in Heqr3.
-          destruct Heqr3 as (pf & EQ). subst.
-          simpl in H.
-
-
-          unfold TypeInference.assert_argtypes in Heqr1.
-
-          rewrite assert_argtypes'_eq in Heqr1.
-
-          assert (List.length args = List.length (rev s)).
-          {
-            apply result_list_map_length in Heqr0. rewrite <- Heqr0.
-            rewrite rev_length; auto.
-          }
-
-          assert (
-              forall (p : pos_t) (sig : tsig var_t) s,
-                result_list_map (TypeInference.type_action TR Sigma p sig) args = Success s ->
-                forall (Gamma : TypedSemantics.tcontext sig) (UGamma : list (var_t * val)),
-                  gamma_eq sig UGamma Gamma ->
-         forall (sched_log action_log action_log' : Logs.Log TR REnv)
-           (usched_log uaction_log : env_t REnv (fun _ : reg_t => RLog val)),
-         log_eq REnv usched_log sched_log ->
-         log_eq REnv uaction_log action_log ->
-         forall (s0 : context
-         (fun k_tau : var_t * type =>
-          TypedSyntax.action pos_t var_t fn_name_t TR Sigma sig (snd k_tau))
-         (rev (int_argspec ufn))),
-           assert_argtypes' (rev (int_argspec ufn))
-                            (rev (combine (map (TypeInference.actpos p) args) s)) = Success s0 ->
-           List.length args = List.length (rev s) ->
-           TypedSemantics.interp_args'
-             (@TypedSemantics.interp_action pos_t var_t fn_name_t reg_t ext_fn_t TR Sigma REnv tr tsigma)
-             Gamma sched_log action_log s0 =
-           None ->
-
-           fold_right
-          (fun a0 (acc : option (Log * list val * list (var_t * val))) =>
-           let/opt3 action_log0, l0, Gamma0 := acc
-           in (let/opt3 action_log1, v0, Gamma1
-               := interp_action r sigma Gamma0 usched_log action_log0 a0
-               in Some (action_log1, v0 :: l0, Gamma1))) (Some (uaction_log, [], UGamma)) (rev args) =
-           None).
-          {
-            generalize interp_action_correct as IAC. intro IAC.
-            clear - IHua IAC.
-            rewrite <- (rev_involutive args).
-            assert (IHua': forall arg, In arg (rev args) -> PP arg).
-            {
-              intros.
-              eapply IHua.
-              apply In_rev in H.
-              revert arg H.
-              induction args; simpl; intros; eauto. easy.
-              destruct H. subst. lia.
-              eapply IHargs in H. lia. intros. eapply IHua. simpl. lia.
-            } clear IHua. revert IHua'.
-            generalize (rev args) as args'.
-            intros args' IHua' p sig s RLM.
-            apply result_list_map_rev in RLM.
-            rewrite combine_rev.
-            rewrite map_rev. rewrite rev_involutive.
-            revert RLM. rewrite rev_involutive.
-            generalize (rev s) as s'. clear s.
-            rewrite rev_length.
-            revert args' IHua' p sig.
-            generalize (rev (int_argspec ufn)). clear args.
-            induction l; simpl; intros.
-            - destr_in H2; [|now inv H2]. inv H2.
-              apply combine_nil_inv in Heql; eauto. destruct Heql. subst.
-              destruct args'; simpl in *; try congruence. inv H4.
-            - destr_in H2.
-              destr_in H2; [inv H2|].
-              destr_in H2.
-              destr_in H2; [|inv H2].
-              destr_in H2; [|inv H2]. inv H2.
-              destruct args'.
-              + simpl in Heql0. congruence.
-              + simpl in Heql0.
-                destr_in Heql0. congruence. inv Heql0. simpl in *.
-                unfold opt_bind in H4.
-                destr_in RLM; [|inv RLM].
-                destr_in RLM; [|inv RLM]. inv RLM. simpl in *.
-                destr_in H4. destruct p0. destruct p0.
-                * edestruct interp_args_correct as (ual' & res & ug' & FR & Geq & Leq & Geq2).
-                  intros arg IN. intros; eapply IAC.  12: eauto. all:eauto. rewrite FR. simpl.
-                  repeat destr_in H4. inv H4.
-                  destruct s. simpl in *. erewrite IHua'; simpl; eauto.
-                  apply cast_action_eq in Heqr0. destruct Heqr0 as (pf & EQ). subst. simpl in *. eauto.
-                * erewrite IHl; simpl; eauto.
-            - rewrite map_length.
-              apply result_list_map_length in RLM.
-              rewrite ! rev_length in *. auto.
-          }
-          move H at bottom.
-          unfold opt_bind in H.
-          repeat destr_in H; try inv H.
-          *
-            rewrite combine_rev in Heqr1.
-            rewrite <- map_rev in Heqr1.
-            edestruct interp_args_correct as (ual' & res & ug' & FR & Geq & Leq & Geq2).
-            intros arg IN. intros; eapply interp_action_correct. 10:eauto.
-            6: apply result_list_map_rev; eauto. 5: eauto. 9: eauto. all: eauto.
-            rewrite rev_length; auto.
-            rewrite <- fold_left_rev_right. setoid_rewrite FR. simpl.
-            erewrite IHua; simpl; eauto. lia.
-            erewrite combine_map. eauto. reflexivity.
-            rewrite map_length. rewrite H0.
-            rewrite rev_length; auto.
-          * rewrite <- fold_left_rev_right.
-            erewrite H1. reflexivity. 6: eauto. eauto. eauto. all: eauto.
-        - destr_in TA; [|inv TA].
-          inv TA.
-          apply Eqdep_dec.inj_pair2_eq_dec in H2. 2: apply eq_dec. subst. simpl in H.
-          destruct s. simpl in *.
-          eapply IHua; eauto.
-      Qed.
-
-      Lemma log_eq_empty:
-        log_eq REnv log_empty Logs.log_empty.
-      Proof.
-        repeat red.
-        unfold log_empty, Logs.log_empty.
-        intros; repeat rewrite getenv_create. constructor.
-      Qed.
-
-      Lemma interp_rule_correct:
-        forall ua p rl
-               (TA: TypeInference.tc_rule TR Sigma p ua = Success rl)
-               sched_log
-               usched_log
-               (SL: log_eq REnv usched_log sched_log)
-               action_log
-        ,
-          TypedSemantics.interp_rule
-            tr tsigma
-            sched_log rl = Some (action_log) ->
-          exists uaction_log,
-            interp_rule
-              (pos_t:=pos_t)
-              (fn_name_t := fn_name_t)
-              r sigma usched_log ua = Some (uaction_log)
-            /\ log_eq REnv uaction_log action_log
-      .
-      Proof.
-        intros.
-        unfold TypeInference.tc_rule in TA.
-        unfold TypeInference.tc_action in TA.
-        destr_in TA; [|inv TA].
-        destruct s; simpl in *.
-        apply cast_action_eq in TA. destruct TA as (pp & EQ).
-        subst. simpl in *.
-        unfold TypedSemantics.interp_rule in H.
-        destr_in H; [|inv H].
-        destruct p0. destruct p0. inv H.
-        unfold interp_rule.
-        edestruct interp_action_correct as (ual' & ug' & IA & LE & GE).
-        eauto. constructor. 3: eauto. apply SL.
-        apply log_eq_empty.
-        rewrite IA.
-        eexists; split; eauto.
-      Qed.
-
-      Lemma interp_rule_none:
-        forall ua p rl
-               (TA: TypeInference.tc_rule TR Sigma p ua = Success rl)
-               sched_log
-               usched_log
-               (SL: log_eq REnv usched_log sched_log)
-        ,
-          TypedSemantics.interp_rule
-            tr tsigma
-            sched_log rl = None ->
-            interp_rule
-              (pos_t:=pos_t)
-              (fn_name_t := fn_name_t)
-              r sigma usched_log ua = None.
-      Proof.
-        intros.
-        unfold TypeInference.tc_rule in TA.
-        unfold TypeInference.tc_action in TA.
-        destr_in TA; [|inv TA].
-        destruct s; simpl in *.
-        apply cast_action_eq in TA. destruct TA as (pp & EQ).
-        subst. simpl in *.
-        unfold TypedSemantics.interp_rule in H.
-        repeat destr_in H; [inv H|].
-        unfold interp_rule.
-        erewrite interp_action_none; eauto. constructor.
-        apply log_eq_empty.
-      Qed.
-
-      Context {rule_name_t: Type}.
-      Lemma interp_scheduler'_correct:
-        forall (urules: rule_name_t -> uaction)
-               (rules: rule_name_t -> TypedSyntax.rule pos_t var_t fn_name_t TR Sigma)
-               (TC: forall rnt,
-                   exists p,
-                     TypeInference.tc_rule TR Sigma p (urules rnt) = Success (rules rnt)
-               ),
-        forall s l1 ul1 l2,
-          log_eq REnv ul1 l1 ->
-          TypedSemantics.interp_scheduler' tr tsigma rules l1 s = l2 ->
-          exists ul2,
-            interp_scheduler' r sigma urules ul1 s = ul2 /\
-            log_eq REnv ul2 l2.
-      Proof.
-        induction s; simpl; intros; eauto.
-        - subst. eexists; split; eauto.
-        - destr_in H0.
-          + destruct (TC r0) as (p & TCR).
-            edestruct interp_rule_correct as (l' & EQ1 & EQ2). eauto. 2: eauto. eauto.
-            rewrite EQ1.
-            eapply IHs; eauto.
-            apply log_eq_app; auto.
-          + destruct (TC r0) as (p & TCR).
-            erewrite interp_rule_none; eauto.
-        - destr_in H0.
-          + destruct (TC r0) as (p & TCR).
-            edestruct interp_rule_correct as (l' & EQ1 & EQ2). eauto. 2: eauto. eauto.
-            rewrite EQ1.
-            eapply IHs1; eauto.
-            apply log_eq_app; auto.
-          + destruct (TC r0) as (p & TCR).
-            erewrite interp_rule_none; eauto.
-      Qed.
-
-      Lemma interp_scheduler_correct:
-        forall (urules: rule_name_t -> uaction)
-               (rules: rule_name_t -> TypedSyntax.rule pos_t var_t fn_name_t TR Sigma)
-               (TC: forall rnt,
-                   exists p,
-                     TypeInference.tc_rule TR Sigma p (urules rnt) = Success (rules rnt)
-               ),
-        forall s l2,
-          TypedSemantics.interp_scheduler tr tsigma rules s = l2 ->
-          exists ul2,
-            interp_scheduler r sigma urules s = ul2 /\
-            log_eq REnv ul2 l2.
-      Proof.
-        intros. unfold interp_scheduler, TypedSemantics.interp_scheduler.
-        eapply interp_scheduler'_correct; eauto.
-        apply log_eq_empty.
-      Qed.
-      End Eq.
+  Lemma interp_scheduler_correct:
+    forall
+      (urules: rule_name_t -> uaction)
+      (rules: rule_name_t -> TypedSyntax.rule pos_t var_t fn_name_t TR Sigma)
+      (TC: forall rnt, exists p,
+        TypeInference.tc_rule TR Sigma p (urules rnt) = Success (rules rnt)
+      ),
+    forall s l2, TypedSemantics.interp_scheduler tr tsigma rules s = l2 ->
+    exists ul2, interp_scheduler r sigma urules s = ul2 /\ log_eq REnv ul2 l2.
+  Proof.
+    intros. unfold interp_scheduler, TypedSemantics.interp_scheduler.
+    eapply interp_scheduler'_correct; eauto.
+    apply log_eq_empty.
+  Qed.
+End Eq.
 
 Section Final.
   Context {reg_t: Type}.
@@ -3360,70 +3369,64 @@ Section Final.
   Variable (tsigma: forall f, Sig_denote (Sigma f)).
 
   Hypothesis tsigma_correct:
-    forall f v,
-      sigma f (val_of_value v) = val_of_value (tsigma f v).
+    forall f v, sigma f (val_of_value v) = val_of_value (tsigma f v).
 
-      Lemma latest_write_eq:
-        forall ulog log,
-          log_eq (TR:=TR) REnv ulog log ->
-          forall idx,
-            option_map val_of_value (Logs.latest_write log idx) =
-            latest_write ulog idx.
-      Proof.
-        unfold Logs.latest_write, latest_write.
-        intros.
-        apply log_find_eq. auto.
-        intros.
-        red in H0. intuition.
-        destruct ule, le; simpl in *. subst.
-        destr_in val1. reflexivity. simpl. congruence.
-      Qed.
+  Lemma latest_write_eq:
+    forall ulog log, log_eq (TR:=TR) REnv ulog log -> forall idx,
+      option_map val_of_value (Logs.latest_write log idx)
+      = latest_write ulog idx.
+  Proof.
+    unfold Logs.latest_write, latest_write.
+    intros.
+    apply log_find_eq. auto.
+    intros.
+    red in H0. intuition.
+    destruct ule, le; simpl in *. subst.
+    destr_in val1. reflexivity. simpl. congruence.
+  Qed.
 
-Lemma log_eq_commit_update:
-  forall ul l,
-    log_eq REnv ul l ->
-    env_t_R (fun (i : reg_t) (uv : val) (v : TR i) => uv = val_of_value v) REnv
-            (create REnv
-                    (fun k : reg_t =>
-                       match latest_write ul k with
-                       | Some v => v
-                       | None => getenv REnv r k
-                       end))
-            (create REnv
-                    (fun k : reg_t =>
-                       match Logs.latest_write l k with
-                       | Some v => v
-                       | None => getenv REnv tr k
-                       end)).
-Proof.
-  intros.
-  red. intros.
-  rewrite !getenv_create.
-  erewrite <- latest_write_eq. 2: eauto.
-  destruct (Logs.latest_write) eqn:?; simpl. auto.
-  apply rtr.
-Qed.
-
-Lemma interp_cycle_correct:
-  forall
-    (urules: rule_name_t -> uaction pos_t var_t fn_name_t reg_t ext_fn_t)
-         (rules: rule_name_t -> TypedSyntax.rule pos_t var_t fn_name_t TR Sigma)
-         (TC: forall rnt,
-             exists p,
-               TypeInference.tc_rule TR Sigma p (urules rnt) = Success (rules rnt)
-         ),
-  forall s,
+  Lemma log_eq_commit_update:
+    forall ul l, log_eq REnv ul l ->
     env_t_R
-      (fun i uv v => uv = val_of_value (tau:=TR i) v)
-      REnv
+      (fun (i : reg_t) (uv : val) (v : TR i) => uv = val_of_value v) REnv
+      (create REnv (fun k : reg_t =>
+        match latest_write ul k with
+        | Some v => v
+        | None => getenv REnv r k
+        end
+      ))
+      (create REnv (fun k : reg_t =>
+        match Logs.latest_write l k with
+        | Some v => v
+        | None => getenv REnv tr k
+        end
+      )).
+  Proof.
+    intros.
+    red. intros.
+    rewrite !getenv_create.
+    erewrite <- latest_write_eq. 2: eauto.
+    destruct (Logs.latest_write) eqn:?; simpl. auto.
+    apply rtr.
+  Qed.
+
+  Lemma interp_cycle_correct:
+    forall
+      (urules: rule_name_t -> uaction pos_t var_t fn_name_t reg_t ext_fn_t)
+      (rules: rule_name_t -> TypedSyntax.rule pos_t var_t fn_name_t TR Sigma)
+      (TC: forall rnt, exists p,
+        TypeInference.tc_rule TR Sigma p (urules rnt) = Success (rules rnt)
+      ),
+    forall s,
+    env_t_R
+      (fun i uv v => uv = val_of_value (tau:=TR i) v) REnv
       (interp_cycle r sigma urules s)
       (TypedSemantics.interp_cycle tsigma rules s tr).
-Proof.
-  unfold interp_cycle, TypedSemantics.interp_cycle. intros.
-  unfold commit_update, Logs.commit_update.
-  apply log_eq_commit_update.
-  edestruct @interp_scheduler_correct as (l2 & EQ & LEQ); eauto.
-  subst.  eauto.
-Qed.
-
+  Proof.
+    unfold interp_cycle, TypedSemantics.interp_cycle. intros.
+    unfold commit_update, Logs.commit_update.
+    apply log_eq_commit_update.
+    edestruct @interp_scheduler_correct as (l2 & EQ & LEQ); eauto.
+    subst.  eauto.
+  Qed.
 End Final.
